src/Init/Data/String/Pattern/Basic.lean
@@ -112,12 +112,12 @@ def memcmpSlice (lhs rhs : Slice) (lstart : String.Pos.Raw) (rstart : String.Pos
     (by
       have := lhs.startInclusive_le_endExclusive
       have := lhs.endExclusive.isValid.le_utf8ByteSize
-      simp [ValidPos.le_iff, Pos.Raw.le_iff, Slice.utf8ByteSize_eq] at *
+      simp [Pos.le_iff, Pos.Raw.le_iff, Slice.utf8ByteSize_eq] at *
       omega)
     (by
       have := rhs.startInclusive_le_endExclusive
       have := rhs.endExclusive.isValid.le_utf8ByteSize
-      simp [ValidPos.le_iff, Pos.Raw.le_iff, Slice.utf8ByteSize_eq] at *
+      simp [Pos.le_iff, Pos.Raw.le_iff, Slice.utf8ByteSize_eq] at *
       omega)
 
 end Internal
